add sanity checks

Examples/MerkleTree/SecurityTheorems.lean
@@ -8,6 +8,8 @@ import Examples.MerkleTree.Instance
 
 namespace DY.Example.MerkleTree
 
+section SecurityTheorems
+
 theorem client_authentication
   (server: Participant)
   (element: Bytes)
@@ -32,5 +34,117 @@ info: 'DY.Example.MerkleTree.client_authentication' depends on axioms: [propext,
 -/
 #guard_msgs in
 #print axioms client_authentication
+
+end SecurityTheorems
+
+section SanityChecks
+
+def honest: Traceful Unit := do
+  let (_, pkHandle, skHandle) ← LongTermKeys.generateKeyPair "MerkleTree PKI" "Bob" -- 4
+  let msgHandle0 ← Network.sendMessage (Literal.literalToBytes "foo 0".toByteArray) -- 1
+  let msgHandle1 ← Network.sendMessage (Literal.literalToBytes "bar 1".toByteArray) -- 1
+  let msgHandle2 ← Network.sendMessage (Literal.literalToBytes "baz 2".toByteArray) -- 1
+  let msgHandle3 ← Network.sendMessage (Literal.literalToBytes "qux 3".toByteArray) -- 1
+  let msgHandle4 ← Network.sendMessage (Literal.literalToBytes "quux 4".toByteArray) -- 1
+  let (msgSigHandle, stHandle) ← Server.authenticate "Bob" [msgHandle0, msgHandle1, msgHandle2, msgHandle3, msgHandle4] skHandle -- 8
+  let msgInclHandle ← Server.proveInclusion "Bob" 3 stHandle -- 1
+  Client.checkInclusion "Bob" msgSigHandle msgInclHandle pkHandle -- 1
+  return ()
+
+theorem honest_PreservesReachability
+  : honest.PreservesReachability reachability
+:= by
+  unfold Traceful.PreservesReachability
+  intro tr h_tr
+  unfold honest
+  apply Traceful.PreservesReachabilityFrom_bind
+  · assumption
+  · apply Traceful.PreservesReachabilityFrom_base (LongTermKeys.generateKeyPair.reachability "MerkleTree PKI")
+    simp [LongTermKeys.generateKeyPair.reachability]
+  intro ⟨ _, pkHandle, skHandle ⟩ tr h_tr h_le
+  dsimp only
+
+  apply Traceful.PreservesReachabilityFrom_bind
+  · assumption
+  · apply Traceful.PreservesReachabilityFrom_base (Network.reachability)
+    simp [Literal.attacker_knows_literalToBytes]
+  intro msgHandle1 tr h_tr tr_le
+  dsimp only
+
+  apply Traceful.PreservesReachabilityFrom_bind
+  · assumption
+  · apply Traceful.PreservesReachabilityFrom_base (Network.reachability)
+    simp [Literal.attacker_knows_literalToBytes]
+  intro msgHandle2 tr h_tr tr_le
+  dsimp only
+
+  apply Traceful.PreservesReachabilityFrom_bind
+  · assumption
+  · apply Traceful.PreservesReachabilityFrom_base (Network.reachability)
+    simp [Literal.attacker_knows_literalToBytes]
+  intro msgHandle3 tr h_tr tr_le
+  dsimp only
+
+  apply Traceful.PreservesReachabilityFrom_bind
+  · assumption
+  · apply Traceful.PreservesReachabilityFrom_base (Network.reachability)
+    simp [Literal.attacker_knows_literalToBytes]
+  intro msgHandle4 tr h_tr tr_le
+  dsimp only
+
+  apply Traceful.PreservesReachabilityFrom_bind
+  · assumption
+  · apply Traceful.PreservesReachabilityFrom_base (Network.reachability)
+    simp [Literal.attacker_knows_literalToBytes]
+  intro msgHandle5 tr h_tr tr_le
+  dsimp only
+
+  apply Traceful.PreservesReachabilityFrom_bind
+  · assumption
+  · apply Traceful.PreservesReachabilityFrom_base (Server.authenticate.reachability) _ ("Bob", [msgHandle1, msgHandle2, msgHandle3, msgHandle4, msgHandle5], skHandle)
+    simp [Server.authenticate.reachability]
+  intro ⟨ msgSigHandle, stHandle ⟩ tr h_tr h_le
+  dsimp only
+
+  apply Traceful.PreservesReachabilityFrom_bind
+  · assumption
+  · apply Traceful.PreservesReachabilityFrom_base (Server.proveInclusion.reachability) _ ("Bob", 3, stHandle)
+    simp [Server.proveInclusion.reachability]
+  intro msgInclHandle tr h_tr h_le
+  dsimp only
+
+  apply Traceful.PreservesReachabilityFrom_bind
+  · assumption
+  · apply Traceful.PreservesReachabilityFrom_base (Client.checkInclusion.reachability) _ ("Bob", msgSigHandle, msgInclHandle, pkHandle)
+    simp [Client.checkInclusion.reachability]
+  intro _ tr h_tr h_le
+
+  apply Traceful.PreservesReachabilityFrom_pure
+
+theorem sanity_check:
+  ∃ tr: ExecTrace,
+    tr.Reachable reachability ∧
+    ∃ (t1 t2: Nat) (msg: Bytes),
+      t1 < t2 ∧
+      tr.EventLoggedAt (TheEvent.ServerAuthenticated "Bob" msg) t1 ∧
+      tr.EventLoggedAt (TheEvent.ClientAccept "Bob" msg) t2
+:= by
+  refine ⟨ (honest.run (Trace.nil)).snd, ?_ ⟩
+  apply And.intro
+  · exact honest_PreservesReachability Trace.nil (Trace.ReachableFrom.Base)
+  refine ⟨ 12, 18, (Literal.literalToBytes "qux 3".toByteArray), ?_ ⟩
+  simp only [DY.Trace.EventLoggedAt_eq_getEventAt]
+  native_decide
+
+/--
+info: 'DY.Example.MerkleTree.sanity_check' depends on axioms: [propext,
+ Classical.choice,
+ Quot.sound,
+ sanity_check._native.native_decide.ax_1_1]
+-/
+#guard_msgs in
+#print axioms sanity_check
+
+end SanityChecks
 
 end DY.Example.MerkleTree
